{
 "cells": [
  {
   "cell_type": "raw",
   "id": "5cae85d7-17b0-4a31-8d6d-35b5d390e062",
   "metadata": {},
   "source": [
    "1. Find the value of T(2) for the recurrence relation T(n) = 3T(n-1) + 12n, given that T(0)=5."
   ]
  },
  {
   "cell_type": "raw",
   "id": "01d4666b-570a-484a-9e9c-944e45924f5e",
   "metadata": {},
   "source": [
    "To find the value of \\( T(2) \\) for the recurrence relation \\( T(n) = 3T(n-1) + 12n \\) with the initial condition \\( T(0) = 5 \\), we can follow these steps:\n",
    "\n",
    "1. Calculate ( T(1) ) using ( T(0) ).\n",
    "2. Calculate ( T(2) ) using ( T(1) ).\n",
    "\n",
    "First, let's calculate ( T(1)):\n",
    "T(1) = 3T(0) + 12.1\n",
    "\n",
    "Substitute ( T(0) = 5 ):\n",
    "\n",
    "T(1) = 3.5 + 12 = 15 + 12 = 27\n",
    "\n",
    "Next, calculate ( T(2) ):\n",
    "\n",
    "T(2) = 3T(1) + 12.2 ]\n",
    "\n",
    "Substitute ( T(1) = 27):\n",
    "\n",
    "T(2) = 3.27 + 24 = 81 + 24 = 105 \n",
    "\n",
    "So, the value of ( T(2) ) is ( 105 )."
   ]
  },
  {
   "cell_type": "raw",
   "id": "4738599d-d88e-44e9-ada0-07d4431cc55b",
   "metadata": {},
   "source": [
    "2. Given a recurrence relation, solve it using the substitution method:\n",
    "a. T(n) = T(n-1) + c\n",
    "b. T(n) = 2T(n/2) + n\n",
    "c. T(n) = 2T(n/2) + c\n",
    "d. T(n) = T(n/2) + c"
   ]
  },
  {
   "cell_type": "raw",
   "id": "19fbb64d-ae46-4cce-985c-9adc62ed596e",
   "metadata": {},
   "source": [
    "Let's solve each recurrence relation using the substitution method.\n",
    "\n",
    "a. T(n) = T(n-1) + c\n",
    "\n",
    "This is a simple linear recurrence. We will solve it by expanding the recurrence.\n",
    "\n",
    "T(n) = T(n-1) + c \n",
    "     = (T(n-2) + c) + c \n",
    "     = T(n-2) + 2c \n",
    "     = .....\n",
    "     = T(n-k) + kc\n",
    "\n",
    "Setting ( k = n ):\n",
    "\n",
    "T(n) = T(0) + nc\n",
    "\n",
    "So, the solution is: T(n) = T(0) + nc\n",
    "\n",
    "b. T(n) = 2T(n/2) + n\n",
    "\n",
    "This is a divide-and-conquer recurrence, which we will solve using the recursion tree method or the Master Theorem. Here, we will use the Master Theorem.\n",
    "\n",
    "The recurrence b. T(n) = 2T(n/2) + n fits the form (T(n) = aT(n/b) + f(n), where ( a = 2), ( b = 2), and ( f(n) = n).\n",
    "\n",
    "Using the Master Theorem:\n",
    "\n",
    "1. ( a = 2 )\n",
    "2. ( b = 2)\n",
    "3. ( f(n) = n )\n",
    "4. ( log_b a = log_2 2 = 1)\n",
    "\n",
    "Since ( f(n) = n =Theta(n^c)) where ( c = 1 ), we compare ( c ) with ( log_b a ):\n",
    "\n",
    "- If ( f(n) = Theta(n^{log_b a}) ), then ( T(n) = Theta(n^{log_b a} log n) ).\n",
    "\n",
    "Here, ( c =log_b a ), so: T(n) = Theta(n log n)\n",
    "\n",
    "c. T(n) = 2T(n/2) + c\n",
    "\n",
    "This is another divide-and-conquer recurrence. We'll use the Master Theorem again.\n",
    "\n",
    "The recurrence ( T(n) = 2T(n/2) + c ) fits the form ( T(n) = aT(n/b) + f(n) ), where ( a = 2 ), ( b = 2 ), and ( f(n) = c ) (a constant).\n",
    "\n",
    "Using the Master Theorem:\n",
    "\n",
    "1. ( a = 2 )\n",
    "2. ( b = 2 )\n",
    "3. ( f(n) = c = Theta(1) )\n",
    "4. ( log_b a = log_2 2 = 1 )\n",
    "\n",
    "Since ( f(n) = Theta(n^0) ) and ( log_b a = 1 ):\n",
    "\n",
    "- If ( f(n) = O(n^c) ) where ( c < log_b a ), then ( T(n) = Theta(n^{log_b a}) ).\n",
    "\n",
    "Here, ( 0 < 1 ): T(n) = Theta(n)\n",
    "\n",
    "d. T(n) = T(n/2) + c\n",
    "\n",
    "This recurrence is simpler than the previous ones. We solve it using the iterative method.\n",
    "\n",
    "T(n) = T(n/2) + c \n",
    "     = (T(n/4) + c) + c \n",
    "     = T(n/4) + 2c \n",
    "     = (T(n/8) + c) + 2c \n",
    "     = T(n/8) + 3c \n",
    "     = .....\n",
    "     = T(n/2^k) + kc\n",
    "\n",
    "\n",
    "Setting ( n/2^k = 1 ):\n",
    "n = 2^k implies k = log_2 n\n",
    "\n",
    "Substitute ( k = log_2 n ):\n",
    "T(n) = T(1) + c \\log_2 n\n",
    "\n",
    "Assuming ( T(1) ) is a constant ( T_0 ):\n",
    "T(n) = T_0 + c \\log_2 n\n",
    "\n",
    "So, the solution is: T(n) = Theta(\\log n)"
   ]
  },
  {
   "cell_type": "raw",
   "id": "b87b5863-8f8b-4ec4-877f-b3a5bf4612a8",
   "metadata": {},
   "source": [
    "3. Given a rec%rrence relation, solve it %sing the rec%rsive tree approach:\n",
    "a. T(n) = 2T(n-1) +1\n",
    "b. T(n) = 2T(n/2) + n"
   ]
  },
  {
   "cell_type": "raw",
   "id": "a7d1eb0a-293c-4cb6-ac8f-e85a72749705",
   "metadata": {},
   "source": [
    "a. T(n) = 2T(n-1) +1\n",
    "\n",
    "- Tree Depth: ( n )\n",
    "- Cost per Level: ( 1, 2, 4,......, 2^{n-1} )\n",
    "- Total Cost: ( 2^n - 1 )\n",
    "\n",
    "Solution: ({O}(2^n))\n",
    "\n",
    "b. T(n) = 2T(n/2) + n\n",
    "\n",
    "- Tree Depth: (log_2{n})\n",
    "- Cost per Level: ( n )\n",
    "- Total Cost: ( n log_2{n} )\n",
    "\n",
    "Solution: ({O}(nlog n))"
   ]
  }
 ],
 "metadata": {
  "kernelspec": {
   "display_name": "Python 3 (ipykernel)",
   "language": "python",
   "name": "python3"
  },
  "language_info": {
   "codemirror_mode": {
    "name": "ipython",
    "version": 3
   },
   "file_extension": ".py",
   "mimetype": "text/x-python",
   "name": "python",
   "nbconvert_exporter": "python",
   "pygments_lexer": "ipython3",
   "version": "3.10.8"
  }
 },
 "nbformat": 4,
 "nbformat_minor": 5
}
